<?xml version="1.0"?>
<rdf:RDF xmlns="http://www.semanticweb.org/bertelt/ontologies/2019/8/untitled-ontology-4#"
     xml:base="http://www.semanticweb.org/bertelt/ontologies/2019/8/untitled-ontology-4"
     xmlns:owl="http://www.w3.org/2002/07/owl#"
     xmlns:rdf="http://www.w3.org/1999/02/22-rdf-syntax-ns#"
     xmlns:xml="http://www.w3.org/XML/1998/namespace"
     xmlns:xsd="http://www.w3.org/2001/XMLSchema#"
     xmlns:rdfs="http://www.w3.org/2000/01/rdf-schema#"
     xmlns:untitled-ontology-4="http://www.semanticweb.org/bertelt/ontologies/2019/8/untitled-ontology-4#">
    <owl:Ontology rdf:about="http://www.semanticweb.org/bertelt/ontologies/2019/8/cyclistDB"/>
    


    <!-- 
    ///////////////////////////////////////////////////////////////////////////////////////
    //
    // Object Properties
    //
    ///////////////////////////////////////////////////////////////////////////////////////
     -->

    


    <!-- http://www.semanticweb.org/bertelt/ontologies/2019/8/cyclistDB#Has_Rider -->

    <owl:ObjectProperty rdf:about="http://www.semanticweb.org/bertelt/ontologies/2019/8/cyclistDB#Has_Rider">
        <owl:inverseOf rdf:resource="http://www.semanticweb.org/bertelt/ontologies/2019/8/cyclistDB#Rides_For"/>
        <rdf:type rdf:resource="http://www.w3.org/2002/07/owl#AsymmetricProperty"/>
        <rdfs:domain rdf:resource="http://www.semanticweb.org/bertelt/ontologies/2019/8/cyclistDB#Team"/>
        <rdfs:range rdf:resource="http://www.semanticweb.org/bertelt/ontologies/2019/8/cyclistDB#Rider"/>
        <rdfs:comment>Relation from Team to Rider, where Team has Rider.
Inverse of &quot;Rider_For&quot; relation.</rdfs:comment>
    </owl:ObjectProperty>
    


    <!-- http://www.semanticweb.org/bertelt/ontologies/2019/8/cyclistDB#Rides_For -->

    <owl:ObjectProperty rdf:about="http://www.semanticweb.org/bertelt/ontologies/2019/8/cyclistDB#Rides_For">
        <rdf:type rdf:resource="http://www.w3.org/2002/07/owl#FunctionalProperty"/>
        <rdf:type rdf:resource="http://www.w3.org/2002/07/owl#AsymmetricProperty"/>
        <rdfs:domain rdf:resource="http://www.semanticweb.org/bertelt/ontologies/2019/8/cyclistDB#Rider"/>
        <rdfs:range rdf:resource="http://www.semanticweb.org/bertelt/ontologies/2019/8/cyclistDB#Team"/>
        <rdfs:comment>Relation from Rider to Team, where Rider rides for Team.
Inverse relation of &quot;Has_Rider&quot;.</rdfs:comment>
    </owl:ObjectProperty>
    


    <!-- http://www.semanticweb.org/bertelt/ontologies/2019/8/cyclistDB#Sponsored_By -->

    <owl:ObjectProperty rdf:about="http://www.semanticweb.org/bertelt/ontologies/2019/8/cyclistDB#Sponsored_By">
        <owl:inverseOf rdf:resource="http://www.semanticweb.org/bertelt/ontologies/2019/8/cyclistDB#Sponsors"/>
        <rdf:type rdf:resource="http://www.w3.org/2002/07/owl#AsymmetricProperty"/>
        <rdfs:domain rdf:resource="http://www.semanticweb.org/bertelt/ontologies/2019/8/cyclistDB#Team"/>
        <rdfs:range rdf:resource="http://www.semanticweb.org/bertelt/ontologies/2019/8/cyclistDB#Sponsor"/>
        <rdfs:comment>Relation from Team to Sponsor, where Team Sponsored_By Sponsor.
Inverse relation of  &quot;Sponsors&quot;.</rdfs:comment>
    </owl:ObjectProperty>
    


    <!-- http://www.semanticweb.org/bertelt/ontologies/2019/8/cyclistDB#Sponsors -->

    <owl:ObjectProperty rdf:about="http://www.semanticweb.org/bertelt/ontologies/2019/8/cyclistDB#Sponsors">
        <rdf:type rdf:resource="http://www.w3.org/2002/07/owl#AsymmetricProperty"/>
        <rdfs:domain rdf:resource="http://www.semanticweb.org/bertelt/ontologies/2019/8/cyclistDB#Sponsor"/>
        <rdfs:range rdf:resource="http://www.semanticweb.org/bertelt/ontologies/2019/8/cyclistDB#Team"/>
        <rdfs:comment>Relation from Sponsor to Team, where Sponsor Sponsors Team.
Inverse relation of  &quot;Sponsored_By&quot;.</rdfs:comment>
    </owl:ObjectProperty>
    


    <!-- 
    ///////////////////////////////////////////////////////////////////////////////////////
    //
    // Data properties
    //
    ///////////////////////////////////////////////////////////////////////////////////////
     -->

    


    <!-- http://www.semanticweb.org/bertelt/ontologies/2019/8/cyclistDB#BirthDate -->

    <owl:DatatypeProperty rdf:about="http://www.semanticweb.org/bertelt/ontologies/2019/8/cyclistDB#BirthDate">
        <rdfs:subPropertyOf rdf:resource="http://www.w3.org/2002/07/owl#topDataProperty"/>
        <rdfs:domain rdf:resource="http://www.semanticweb.org/bertelt/ontologies/2019/8/cyclistDB#Rider"/>
        <rdfs:range rdf:resource="http://www.w3.org/2001/XMLSchema#string"/>
        <rdfs:comment>Property of the Rider class with a date in format yyy-mm-dd representing the date of birth as a string.
Can be null.</rdfs:comment>
    </owl:DatatypeProperty>
    


    <!-- http://www.semanticweb.org/bertelt/ontologies/2019/8/cyclistDB#BirthPlace -->

    <owl:DatatypeProperty rdf:about="http://www.semanticweb.org/bertelt/ontologies/2019/8/cyclistDB#BirthPlace">
        <rdfs:subPropertyOf rdf:resource="http://www.w3.org/2002/07/owl#topDataProperty"/>
        <rdfs:domain rdf:resource="http://www.semanticweb.org/bertelt/ontologies/2019/8/cyclistDB#Rider"/>
        <rdfs:range rdf:resource="http://www.w3.org/2001/XMLSchema#string"/>
        <rdfs:comment>Property of the Rider class with a string representing the place of birth.
Can be null.</rdfs:comment>
    </owl:DatatypeProperty>
    


    <!-- http://www.semanticweb.org/bertelt/ontologies/2019/8/cyclistDB#RiderType -->

    <owl:DatatypeProperty rdf:about="http://www.semanticweb.org/bertelt/ontologies/2019/8/cyclistDB#RiderType">
        <rdfs:subPropertyOf rdf:resource="http://www.w3.org/2002/07/owl#topDataProperty"/>
        <rdfs:domain rdf:resource="http://www.semanticweb.org/bertelt/ontologies/2019/8/cyclistDB#Rider"/>
        <rdfs:range rdf:resource="http://www.w3.org/2001/XMLSchema#string"/>
        <rdfs:comment>Genre of the Cyclists, property of the Rider class.
Can be: sprinter, climber, tt, gc, classic or null.</rdfs:comment>
    </owl:DatatypeProperty>
    


    <!-- http://www.semanticweb.org/bertelt/ontologies/2019/8/cyclistDB#FullName -->

    <owl:DatatypeProperty rdf:about="http://www.semanticweb.org/bertelt/ontologies/2019/8/cyclistDB#FullName">
        <rdfs:subPropertyOf rdf:resource="http://www.w3.org/2002/07/owl#topDataProperty"/>
        <rdfs:domain rdf:resource="http://www.semanticweb.org/bertelt/ontologies/2019/8/cyclistDB#Rider"/>
        <rdfs:range rdf:resource="http://www.w3.org/2001/XMLSchema#string"/>
        <rdfs:comment>Property for Rider class with a string that represents the full name.</rdfs:comment>
    </owl:DatatypeProperty>
    


    <!-- http://www.semanticweb.org/bertelt/ontologies/2019/8/cyclistDB#GivenName -->

    <owl:DatatypeProperty rdf:about="http://www.semanticweb.org/bertelt/ontologies/2019/8/cyclistDB#GivenName">
        <rdfs:subPropertyOf rdf:resource="http://www.w3.org/2002/07/owl#topDataProperty"/>
        <rdfs:domain rdf:resource="http://www.semanticweb.org/bertelt/ontologies/2019/8/cyclistDB#Rider"/>
        <rdfs:range rdf:resource="http://www.w3.org/2001/XMLSchema#string"/>
        <rdfs:comment>The given name / first name of a Rider.
Cannot be null.</rdfs:comment>
    </owl:DatatypeProperty>
    


    <!-- http://www.semanticweb.org/bertelt/ontologies/2019/8/cyclistDB#Height -->

    <owl:DatatypeProperty rdf:about="http://www.semanticweb.org/bertelt/ontologies/2019/8/cyclistDB#Height">
        <rdfs:subPropertyOf rdf:resource="http://www.w3.org/2002/07/owl#topDataProperty"/>
        <rdfs:domain rdf:resource="http://www.semanticweb.org/bertelt/ontologies/2019/8/cyclistDB#Rider"/>
        <rdfs:range rdf:resource="http://www.w3.org/2001/XMLSchema#double"/>
        <rdfs:comment>Height property of the Rider class, with double value representing the height in m.
Can be null.</rdfs:comment>
    </owl:DatatypeProperty>
    


    <!-- http://www.semanticweb.org/bertelt/ontologies/2019/8/cyclistDB#Nationality -->

    <owl:DatatypeProperty rdf:about="http://www.semanticweb.org/bertelt/ontologies/2019/8/cyclistDB#Nationality">
        <rdfs:subPropertyOf rdf:resource="http://www.w3.org/2002/07/owl#topDataProperty"/>
        <rdfs:domain>
            <owl:Class>
                <owl:unionOf rdf:parseType="Collection">
                    <rdf:Description rdf:about="http://www.semanticweb.org/bertelt/ontologies/2019/8/cyclistDB#Rider"/>
                    <rdf:Description rdf:about="http://www.semanticweb.org/bertelt/ontologies/2019/8/cyclistDB#Team"/>
                </owl:unionOf>
            </owl:Class>
        </rdfs:domain>
        <rdfs:range rdf:resource="http://www.w3.org/2001/XMLSchema#string"/>
        <rdfs:comment>Property of the Rider class with a string that represents the nationality.
Cannot be null.</rdfs:comment>
    </owl:DatatypeProperty>
    


    <!-- http://www.semanticweb.org/bertelt/ontologies/2019/8/cyclistDB#Status -->

    <owl:DatatypeProperty rdf:about="http://www.semanticweb.org/bertelt/ontologies/2019/8/cyclistDB#Status">
        <rdfs:subPropertyOf rdf:resource="http://www.w3.org/2002/07/owl#topDataProperty"/>
        <rdfs:domain rdf:resource="http://www.semanticweb.org/bertelt/ontologies/2019/8/cyclistDB#Team"/>
        <rdfs:range rdf:resource="http://www.w3.org/2001/XMLSchema#string"/>
        <rdfs:comment>Status property of the Team Class, which specifies if a team is a WorldTeam (WT), ProContinental (PCT), Continental (CT) or UCI Women (UCI) (not included in data set).
Cannot be null.</rdfs:comment>
    </owl:DatatypeProperty>
    


    <!-- http://www.semanticweb.org/bertelt/ontologies/2019/8/cyclistDB#Surname -->

    <owl:DatatypeProperty rdf:about="http://www.semanticweb.org/bertelt/ontologies/2019/8/cyclistDB#Surname">
        <rdfs:subPropertyOf rdf:resource="http://www.w3.org/2002/07/owl#topDataProperty"/>
        <rdfs:domain rdf:resource="http://www.semanticweb.org/bertelt/ontologies/2019/8/cyclistDB#Rider"/>
        <rdfs:range rdf:resource="http://www.w3.org/2001/XMLSchema#string"/>
        <rdfs:comment>Property of the Rider class with a string representing the surname.
Cannot be null.</rdfs:comment>
    </owl:DatatypeProperty>
    


    <!-- http://www.semanticweb.org/bertelt/ontologies/2019/8/cyclistDB#UCI_rank -->

    <owl:DatatypeProperty rdf:about="http://www.semanticweb.org/bertelt/ontologies/2019/8/cyclistDB#UCI_rank">
        <rdfs:subPropertyOf rdf:resource="http://www.w3.org/2002/07/owl#topDataProperty"/>
        <rdfs:domain rdf:resource="http://www.semanticweb.org/bertelt/ontologies/2019/8/cyclistDB#Rider"/>
        <rdfs:range rdf:resource="http://www.w3.org/2001/XMLSchema#int"/>
        <rdfs:comment>Property of Rider, with integer that represents the UCI rank.
Can be null.</rdfs:comment>
    </owl:DatatypeProperty>
    


    <!-- http://www.semanticweb.org/bertelt/ontologies/2019/8/cyclistDB#URL -->

    <owl:DatatypeProperty rdf:about="http://www.semanticweb.org/bertelt/ontologies/2019/8/cyclistDB#URL">
        <rdfs:subPropertyOf rdf:resource="http://www.w3.org/2002/07/owl#topDataProperty"/>
        <rdfs:domain>
            <owl:Class>
                <owl:unionOf rdf:parseType="Collection">
                    <rdf:Description rdf:about="http://www.semanticweb.org/bertelt/ontologies/2019/8/cyclistDB#Rider"/>
                    <rdf:Description rdf:about="http://www.semanticweb.org/bertelt/ontologies/2019/8/cyclistDB#Sponsor"/>
                    <rdf:Description rdf:about="http://www.semanticweb.org/bertelt/ontologies/2019/8/cyclistDB#Team"/>
                </owl:unionOf>
            </owl:Class>
        </rdfs:domain>
        <rdfs:range rdf:resource="http://www.w3.org/2001/XMLSchema#string"/>
        <rdfs:comment>URL Property containing URL to DBpedia for all classes.</rdfs:comment>
    </owl:DatatypeProperty>
    


    <!-- http://www.semanticweb.org/bertelt/ontologies/2019/8/cyclistDB#Weight -->

    <owl:DatatypeProperty rdf:about="http://www.semanticweb.org/bertelt/ontologies/2019/8/cyclistDB#Weight">
        <rdfs:subPropertyOf rdf:resource="http://www.w3.org/2002/07/owl#topDataProperty"/>
        <rdfs:domain rdf:resource="http://www.semanticweb.org/bertelt/ontologies/2019/8/cyclistDB#Rider"/>
        <rdfs:range rdf:resource="http://www.w3.org/2001/XMLSchema#double"/>
        <rdfs:comment>Property of the Rider class with double representing the weight in kg.
Can also be null.</rdfs:comment>
    </owl:DatatypeProperty>
    


    <!-- http://www.semanticweb.org/bertelt/ontologies/2019/8/cyclistDB#uciCode -->

    <owl:DatatypeProperty rdf:about="http://www.semanticweb.org/bertelt/ontologies/2019/8/cyclistDB#uciCode">
        <rdfs:subPropertyOf rdf:resource="http://www.w3.org/2002/07/owl#topDataProperty"/>
        <rdfs:domain rdf:resource="http://www.semanticweb.org/bertelt/ontologies/2019/8/cyclistDB#Team"/>
        <rdfs:range rdf:resource="http://www.w3.org/2001/XMLSchema#string"/>
        <rdfs:comment>Property of Team, that specifies the three letter string which represents a team.
Cannot be null</rdfs:comment>
    </owl:DatatypeProperty>
    


    <!-- 
    ///////////////////////////////////////////////////////////////////////////////////////
    //
    // Classes
    //
    ///////////////////////////////////////////////////////////////////////////////////////
     -->

    


    <!-- http://www.semanticweb.org/bertelt/ontologies/2019/8/cyclistDB#Bike_Sponsor -->

    <owl:Class rdf:about="http://www.semanticweb.org/bertelt/ontologies/2019/8/cyclistDB#Bike_Sponsor">
        <rdfs:subClassOf rdf:resource="http://www.semanticweb.org/bertelt/ontologies/2019/8/cyclistDB#Sponsor"/>
        <rdfs:comment>Bike Sponsor class that contains the Bike brands that sponsor Teams.
Has the following relations with Team: &quot;Sponsors&quot; and the inverse relation &quot;Sponsored_By&quot;.</rdfs:comment>
    </owl:Class>
    


    <!-- http://www.semanticweb.org/bertelt/ontologies/2019/8/cyclistDB#Rider -->

    <owl:Class rdf:about="http://www.semanticweb.org/bertelt/ontologies/2019/8/cyclistDB#Rider">
        <rdfs:comment>Rider Class with cyclists from 2019.
Has three subclasses that are based on which type of team a rider is in.
Contains the properties: UCI_rank, Height, GivenName, Nationality, CyclistGenre, ProTeam, Surname, BirthDate, BirthPlace and Weight.</rdfs:comment>
    </owl:Class>
    


    <!-- http://www.semanticweb.org/bertelt/ontologies/2019/8/cyclistDB#Sponsor -->

    <owl:Class rdf:about="http://www.semanticweb.org/bertelt/ontologies/2019/8/cyclistDB#Sponsor"/>
    


    <!-- http://www.semanticweb.org/bertelt/ontologies/2019/8/cyclistDB#Team -->

    <owl:Class rdf:about="http://www.semanticweb.org/bertelt/ontologies/2019/8/cyclistDB#Team">
        <rdfs:comment>Team class that contains teams from 2019.
Contains properties: Status, UCI_code and Bike.
Subclasses are the UCI Women (UCI)(not used in data set), UCI Continental (CT), UCI Professional Continental (PCT) and UCI WorldTeam (WT).</rdfs:comment>
    </owl:Class>
    


    <!-- http://www.semanticweb.org/bertelt/ontologies/2019/8/cyclistDB#UCI_Continental -->

    <owl:Class rdf:about="http://www.semanticweb.org/bertelt/ontologies/2019/8/cyclistDB#UCI_Continental">
        <owl:equivalentClass>
            <owl:Class>
                <owl:intersectionOf rdf:parseType="Collection">
                    <rdf:Description rdf:about="http://www.semanticweb.org/bertelt/ontologies/2019/8/cyclistDB#Team"/>
                    <owl:Restriction>
                        <owl:onProperty rdf:resource="http://www.semanticweb.org/bertelt/ontologies/2019/8/cyclistDB#Status"/>
                        <owl:hasValue>CT (2019)</owl:hasValue>
                    </owl:Restriction>
                </owl:intersectionOf>
            </owl:Class>
        </owl:equivalentClass>
        <rdfs:subClassOf rdf:resource="http://www.semanticweb.org/bertelt/ontologies/2019/8/cyclistDB#Team"/>
        <rdfs:comment>UCI Continental is a subclass of the Team Class, where a Team has the Status &quot;CT&quot;.</rdfs:comment>
    </owl:Class>
    


    <!-- http://www.semanticweb.org/bertelt/ontologies/2019/8/cyclistDB#UCI_Continental_Rider -->

    <owl:Class rdf:about="http://www.semanticweb.org/bertelt/ontologies/2019/8/cyclistDB#UCI_Continental_Rider">
        <owl:equivalentClass>
            <owl:Class>
                <owl:intersectionOf rdf:parseType="Collection">
                    <rdf:Description rdf:about="http://www.semanticweb.org/bertelt/ontologies/2019/8/cyclistDB#Rider"/>
                    <owl:Restriction>
                        <owl:onProperty rdf:resource="http://www.semanticweb.org/bertelt/ontologies/2019/8/cyclistDB#Rides_For"/>
                        <owl:someValuesFrom rdf:resource="http://www.semanticweb.org/bertelt/ontologies/2019/8/cyclistDB#UCI_Continental"/>
                    </owl:Restriction>
                </owl:intersectionOf>
            </owl:Class>
        </owl:equivalentClass>
        <rdfs:subClassOf rdf:resource="http://www.semanticweb.org/bertelt/ontologies/2019/8/cyclistDB#Rider"/>
        <rdfs:comment>Subclass of the Rider class, for riders that are part of a UCI Continental team.</rdfs:comment>
    </owl:Class>
    


    <!-- http://www.semanticweb.org/bertelt/ontologies/2019/8/cyclistDB#UCI_Professional_Continental -->

    <owl:Class rdf:about="http://www.semanticweb.org/bertelt/ontologies/2019/8/cyclistDB#UCI_Professional_Continental">
        <owl:equivalentClass>
            <owl:Class>
                <owl:intersectionOf rdf:parseType="Collection">
                    <rdf:Description rdf:about="http://www.semanticweb.org/bertelt/ontologies/2019/8/cyclistDB#Team"/>
                    <owl:Restriction>
                        <owl:onProperty rdf:resource="http://www.semanticweb.org/bertelt/ontologies/2019/8/cyclistDB#Status"/>
                        <owl:hasValue>PCT (2019)</owl:hasValue>
                    </owl:Restriction>
                </owl:intersectionOf>
            </owl:Class>
        </owl:equivalentClass>
        <rdfs:subClassOf rdf:resource="http://www.semanticweb.org/bertelt/ontologies/2019/8/cyclistDB#Team"/>
        <rdfs:comment>UCI Professional Continental is a subclass of the Team Class, where a Team has the Status &quot;PCT&quot;.</rdfs:comment>
    </owl:Class>
    


    <!-- http://www.semanticweb.org/bertelt/ontologies/2019/8/cyclistDB#UCI_Professional_Continental_Rider -->

    <owl:Class rdf:about="http://www.semanticweb.org/bertelt/ontologies/2019/8/cyclistDB#UCI_Professional_Continental_Rider">
        <owl:equivalentClass>
            <owl:Class>
                <owl:intersectionOf rdf:parseType="Collection">
                    <rdf:Description rdf:about="http://www.semanticweb.org/bertelt/ontologies/2019/8/cyclistDB#Rider"/>
                    <owl:Restriction>
                        <owl:onProperty rdf:resource="http://www.semanticweb.org/bertelt/ontologies/2019/8/cyclistDB#Rides_For"/>
                        <owl:someValuesFrom rdf:resource="http://www.semanticweb.org/bertelt/ontologies/2019/8/cyclistDB#UCI_Professional_Continental"/>
                    </owl:Restriction>
                </owl:intersectionOf>
            </owl:Class>
        </owl:equivalentClass>
        <rdfs:subClassOf rdf:resource="http://www.semanticweb.org/bertelt/ontologies/2019/8/cyclistDB#Rider"/>
        <rdfs:comment>Subclass of the Rider class, for riders that are part of a UCI Proffesional Continental team.</rdfs:comment>
    </owl:Class>
    


    <!-- http://www.semanticweb.org/bertelt/ontologies/2019/8/cyclistDB#UCI_WorldTeam -->

    <owl:Class rdf:about="http://www.semanticweb.org/bertelt/ontologies/2019/8/cyclistDB#UCI_WorldTeam">
        <owl:equivalentClass>
            <owl:Class>
                <owl:intersectionOf rdf:parseType="Collection">
                    <rdf:Description rdf:about="http://www.semanticweb.org/bertelt/ontologies/2019/8/cyclistDB#Team"/>
                    <owl:Restriction>
                        <owl:onProperty rdf:resource="http://www.semanticweb.org/bertelt/ontologies/2019/8/cyclistDB#Status"/>
                        <owl:hasValue>WT (2019)</owl:hasValue>
                    </owl:Restriction>
                </owl:intersectionOf>
            </owl:Class>
        </owl:equivalentClass>
        <rdfs:subClassOf rdf:resource="http://www.semanticweb.org/bertelt/ontologies/2019/8/cyclistDB#Team"/>
        <rdfs:comment>UCI WorldTeam is a subclass of the Team Class, where a Team has the Status &quot;WT&quot;.</rdfs:comment>
    </owl:Class>
    


    <!-- http://www.semanticweb.org/bertelt/ontologies/2019/8/cyclistDB#UCI_WorldTeam_Rider -->

    <owl:Class rdf:about="http://www.semanticweb.org/bertelt/ontologies/2019/8/cyclistDB#UCI_WorldTeam_Rider">
        <owl:equivalentClass>
            <owl:Class>
                <owl:intersectionOf rdf:parseType="Collection">
                    <rdf:Description rdf:about="http://www.semanticweb.org/bertelt/ontologies/2019/8/cyclistDB#Rider"/>
                    <owl:Restriction>
                        <owl:onProperty rdf:resource="http://www.semanticweb.org/bertelt/ontologies/2019/8/cyclistDB#Rides_For"/>
                        <owl:someValuesFrom rdf:resource="http://www.semanticweb.org/bertelt/ontologies/2019/8/cyclistDB#UCI_WorldTeam"/>
                    </owl:Restriction>
                </owl:intersectionOf>
            </owl:Class>
        </owl:equivalentClass>
        <rdfs:subClassOf rdf:resource="http://www.semanticweb.org/bertelt/ontologies/2019/8/cyclistDB#Rider"/>
        <rdfs:comment>Subclass of the Rider class, for riders that are part of a UCI WorldTeam.</rdfs:comment>
    </owl:Class>
</rdf:RDF>



<!-- Generated by the OWL API (version 4.5.9.2019-02-01T07:24:44Z) https://github.com/owlcs/owlapi -->

